ExhaleRel.thy
@@ -2,16 +2,13 @@ theory ExhaleRel
   imports ExpRel ExprWfRel TotalViper.ViperBoogieTranslationInterface Simulation
 begin
 
-abbreviation convert_rel
-  where "convert_rel R \<omega>0_\<omega> \<equiv> R (fst \<omega>0_\<omega>) (snd \<omega>0_\<omega>)"
-
 definition exhale_rel :: 
     "('a full_total_state \<Rightarrow> 'a full_total_state \<Rightarrow> 'b nstate \<Rightarrow> bool)
      \<Rightarrow> 'a total_context
         \<Rightarrow> ('a full_total_state \<Rightarrow> bool)
            \<Rightarrow> bigblock list \<Rightarrow> 'b econtext_bpl_general \<Rightarrow> (pure_exp, pure_exp atomic_assert) assert \<Rightarrow> bigblock \<times> cont \<Rightarrow> bigblock \<times> cont \<Rightarrow> bool"
   where "exhale_rel R ctxt_vpr StateCons P ctxt assertion_vpr \<gamma> \<gamma>' \<equiv>
-         rel_general (convert_rel R) (convert_rel R)
+         rel_general (uncurry R) (uncurry R)
            \<comment>\<open>The well-definedness state remains the same\<close>
            (\<lambda> \<omega>0_\<omega> \<omega>0_\<omega>'. (fst \<omega>0_\<omega>) = (fst \<omega>0_\<omega>') \<and> red_exhale ctxt_vpr StateCons (fst \<omega>0_\<omega>) assertion_vpr (snd \<omega>0_\<omega>) (RNormal (snd \<omega>0_\<omega>')))
            (\<lambda> \<omega>0_\<omega>. red_exhale ctxt_vpr StateCons (fst \<omega>0_\<omega>) assertion_vpr (snd \<omega>0_\<omega>) RFailure)
@@ -48,7 +45,7 @@ lemma exhale_rel_normal_elim:
   shows "\<exists>ns'. red_ast_bpl P ctxt (\<gamma>, Normal ns) (\<gamma>', Normal ns') \<and> R \<omega>0 \<omega>' ns'"
   using assms
   unfolding exhale_rel_def rel_general_def
-  by (metis fst_eqD snd_conv)
+  by simp
 
 lemma exhale_rel_failure_elim:
   assumes "exhale_rel R ctxt_vpr StateCons P ctxt assertion_vpr \<gamma> \<gamma>'" and
@@ -57,7 +54,7 @@ lemma exhale_rel_failure_elim:
         shows "\<exists>\<gamma>'. red_ast_bpl P ctxt (\<gamma>, Normal ns) (\<gamma>', Failure)"  
   using assms
   unfolding exhale_rel_def rel_general_def
-  by (metis fst_conv snd_conv surjective_pairing)
+  by simp
 
 subsection \<open>Propagation rules\<close>
 
@@ -65,7 +62,7 @@ lemma exhale_rel_propagate_pre:
   assumes "\<And> \<omega>0 \<omega> ns. R \<omega>0 \<omega> ns \<Longrightarrow> \<exists>ns'. red_ast_bpl P ctxt (\<gamma>0, Normal ns) (\<gamma>1, Normal ns') \<and> R \<omega>0 \<omega> ns'" and
           "exhale_rel R ctxt_vpr StateCons P ctxt assertion_vpr \<gamma>1 \<gamma>2"
         shows "exhale_rel R ctxt_vpr StateCons P ctxt assertion_vpr \<gamma>0 \<gamma>2"
-  using assms(2)
+  using assms rel_propagate_pre
   unfolding exhale_rel_def
   by (auto intro: rel_propagate_pre assms(1))
 
@@ -100,9 +97,11 @@ lemma exhale_rel_imp:
    RhsRel: "exhale_rel R ctxt_vpr StateCons P ctxt A (thn_hd, convert_list_to_cont thn_tl (KSeq next cont)) (next, cont)"
                 (is "exhale_rel R _ _ _ _ _ ?\<gamma>_thn (next, cont)") 
               shows "exhale_rel R ctxt_vpr StateCons P ctxt (assert.Imp cond A) \<gamma>1 (next, cont)"
-  using RhsRel
-  unfolding exhale_rel_def  
-proof (rule rel_general_cond[OF rev_iffD1_def[OF wf_rel_inst_eq_1[OF ExpWfRel] wf_rel_inst_def]] )
+  (*using RhsRel*)
+  unfolding exhale_rel_def 
+  thm rel_general_cond[OF rev_iffD1_def[OF wf_rel_inst_eq_1[OF ExpWfRel] wf_rel_inst_def]]
+  thm uncurry.simps
+proof (simp only: uncurry.simps, rule rel_general_cond[OF rev_iffD1_def[OF wf_rel_inst_eq_1[OF ExpWfRel] wf_rel_inst_def]])
   show "rel_general (\<lambda>\<omega>0_\<omega>. R (fst \<omega>0_\<omega>) (snd \<omega>0_\<omega>)) (\<lambda>\<omega>0_\<omega>. R (fst \<omega>0_\<omega>) (snd \<omega>0_\<omega>)) (\<lambda> \<omega> \<omega>'. \<omega> = \<omega>') (\<lambda>_. False) P ctxt (empty_else_block, convert_list_to_cont [] (KSeq next cont)) (next, cont)"
     apply (rule rel_intro)
     using red_ast_bpl_empty_block_2[OF EmptyElse]
@@ -112,6 +111,14 @@ next
   let ?Success = "\<lambda>\<omega> \<omega>'. fst \<omega> = fst \<omega>' \<and> red_exhale ctxt_vpr StateCons (fst \<omega>) (assert.Imp cond A) (snd \<omega>) (RNormal (snd \<omega>'))"
   let ?SuccessExp = "\<lambda>\<omega> \<omega>'. \<omega> = \<omega>' \<and> (\<exists>v. ctxt_vpr, StateCons, Some (fst \<omega>) \<turnstile> \<langle>cond;snd \<omega>\<rangle> [\<Down>]\<^sub>t Val v)"
   let ?SuccessThn = "\<lambda>\<omega> \<omega>'. fst \<omega> = fst \<omega>' \<and> red_exhale ctxt_vpr StateCons (fst \<omega>) A (snd \<omega>) (RNormal (snd \<omega>'))"
+  let ?Fail ="\<lambda>\<omega>. red_exhale ctxt_vpr StateCons (fst \<omega>) (assert.Imp cond A) (snd \<omega>) RFailure"
+  let ?FailThn = "\<lambda>\<omega>. red_exhale ctxt_vpr StateCons (fst \<omega>) A (snd \<omega>) RFailure"
+  let ?FailExp = "\<lambda>\<omega>. ctxt_vpr, StateCons, Some (fst \<omega>) \<turnstile> \<langle>cond;snd \<omega>\<rangle> [\<Down>]\<^sub>t VFailure"
+
+  show "rel_general (\<lambda>a. R (fst a) (snd a)) (\<lambda>a. R (fst a) (snd a)) ?SuccessThn ?FailThn P ctxt (thn_hd, convert_list_to_cont thn_tl (KSeq next cont)) (next, cont)"
+    using RhsRel
+    unfolding exhale_rel_def
+    by simp
   
   show "\<And> \<omega> \<omega>' ns. ?Success \<omega> \<omega>' \<Longrightarrow> R (fst \<omega>) (snd \<omega>) ns \<Longrightarrow>
                         ?SuccessExp \<omega> \<omega> \<and> \<comment>\<open>implicit assumption that success of conditional does not lead to side effects\<close>
@@ -132,10 +139,6 @@ next
       using exp_rel_vpr_bpl_elim_2[OF ExpRel] Success
       by (metis R prod_eqI val_rel_vpr_bpl.simps(2))
   qed
-
-  let ?Fail ="\<lambda>\<omega>. red_exhale ctxt_vpr StateCons (fst \<omega>) (assert.Imp cond A) (snd \<omega>) RFailure"
-  let ?FailThn = "\<lambda>\<omega>. red_exhale ctxt_vpr StateCons (fst \<omega>) A (snd \<omega>) RFailure"
-  let ?FailExp = "\<lambda>\<omega>. ctxt_vpr, StateCons, Some (fst \<omega>) \<turnstile> \<langle>cond;snd \<omega>\<rangle> [\<Down>]\<^sub>t VFailure"
 
  show "\<And> \<omega> ns. ?Fail \<omega> \<Longrightarrow> R (fst \<omega>) (snd \<omega>) ns \<Longrightarrow> 
                ?FailExp \<omega> \<or>
@@ -170,6 +173,20 @@ definition exhale_field_acc_rel_assms
             ctxt, StateCons, Some \<omega>0 \<turnstile> \<langle>e_r; \<omega>\<rangle> [\<Down>]\<^sub>t Val (VRef r) \<and>
             ctxt, StateCons, Some \<omega>0 \<turnstile> \<langle>e_p; \<omega>\<rangle> [\<Down>]\<^sub>t Val (VPerm p)"
 
+lemma exhale_field_acc_rel_assms_perm_eval:
+  assumes "exhale_field_acc_rel_assms ctxt StateCons e_r f e_p r p \<omega>0 \<omega>"
+  shows "ctxt, StateCons, Some \<omega>0 \<turnstile> \<langle>e_p; \<omega>\<rangle> [\<Down>]\<^sub>t Val (VPerm p)"
+  using assms
+  unfolding exhale_field_acc_rel_assms_def
+  by blast
+
+lemma exhale_field_acc_rel_assms_ref_eval:
+  assumes "exhale_field_acc_rel_assms ctxt StateCons e_r f e_p r p \<omega>0 \<omega>"
+  shows "ctxt, StateCons, Some \<omega>0 \<turnstile> \<langle>e_r; \<omega>\<rangle> [\<Down>]\<^sub>t Val (VRef r)"
+  using assms
+  unfolding exhale_field_acc_rel_assms_def
+  by blast
+
 definition exhale_acc_normal_premise
   where "exhale_acc_normal_premise ctxt StateCons e_r f e_p p r \<omega>0 \<omega> \<omega>' \<equiv>
        exhale_field_acc_rel_assms ctxt StateCons e_r f e_p r p \<omega>0 \<omega>  \<and>
@@ -184,7 +201,7 @@ lemma exhale_field_acc_rel:
     WfRcv: "expr_wf_rel R ctxt_vpr StateCons P ctxt e_rcv_vpr \<gamma> \<gamma>1" and
     WfPerm: "expr_wf_rel R ctxt_vpr StateCons P ctxt e_p \<gamma>1 \<gamma>2" and
     CorrectPermRel:  
-            "\<And>r p. rel_general (convert_rel R) (R' r p)
+            "\<And>r p. rel_general (uncurry R) (R' r p)
                   (\<lambda> \<omega>0_\<omega> \<omega>0_\<omega>'. \<omega>0_\<omega> = \<omega>0_\<omega>' \<and> 
                                   exhale_field_acc_rel_assms ctxt_vpr StateCons e_rcv_vpr f e_p r p (fst \<omega>0_\<omega>) (snd \<omega>0_\<omega>)  \<and>
                                   exhale_field_acc_rel_perm_success ctxt_vpr StateCons (snd \<omega>0_\<omega>) r p f)
@@ -192,7 +209,7 @@ lemma exhale_field_acc_rel:
                            \<not> exhale_field_acc_rel_perm_success ctxt_vpr StateCons  (snd \<omega>0_\<omega>) r p f)
                   P ctxt \<gamma>2 \<gamma>3" and
     
-    UpdExhRel: "\<And>r p. rel_general (R' r p) (convert_rel R) \<comment>\<open>Here, the simulation needs to revert back to R\<close>
+    UpdExhRel: "\<And>r p. rel_general (R' r p) (uncurry R) \<comment>\<open>Here, the simulation needs to revert back to R\<close>
                       (\<lambda> \<omega>0_\<omega> \<omega>0_\<omega>'. exhale_acc_normal_premise ctxt_vpr StateCons e_rcv_vpr f e_p p r (fst \<omega>0_\<omega>) (snd \<omega>0_\<omega>) (snd \<omega>0_\<omega>'))
                       (\<lambda>_. False) 
                       P ctxt \<gamma>3 \<gamma>'"
@@ -212,7 +229,7 @@ proof (rule exhale_rel_intro_2)
       using wf_rel_normal_elim[OF WfPerm R1] red_ast_bpl_transitive
       by blast
 
-    hence R2_conv:"convert_rel R (\<omega>0, \<omega>) ns2"
+    hence R2_conv:"uncurry R (\<omega>0, \<omega>) ns2"
       by simp
 
     have BasicAssms: "exhale_field_acc_rel_assms ctxt_vpr StateCons e_rcv_vpr f e_p r p \<omega>0 \<omega>"
@@ -232,6 +249,8 @@ proof (rule exhale_rel_intro_2)
         using \<open>mh = _\<close> \<open>a = _\<close>
         by blast     
       from this obtain ns3 where Red3: "red_ast_bpl P ctxt (\<gamma>, Normal ns) (\<gamma>3, Normal ns3)" and R3: "R' r p (\<omega>0, \<omega>) ns3"
+        thm rel_success_elim[OF CorrectPermRel] R2_conv
+
         using BasicAssms rel_success_elim[OF CorrectPermRel R2_conv] red_ast_bpl_transitive[OF Red2]
         by (metis fst_eqD snd_eqD)
 
@@ -243,7 +262,7 @@ proof (rule exhale_rel_intro_2)
         
        thus "\<exists>ns'. red_ast_bpl P ctxt (\<gamma>, Normal ns) (\<gamma>', Normal ns') \<and> R \<omega>0 \<omega>' ns'"
          using rel_success_elim[OF UpdExhRel R3] red_ast_bpl_transitive[OF Red3] 
-         by (metis prod.collapse prod.inject)                                        
+         by (metis (no_types, lifting) old.prod.inject prod.collapse uncurry.elims)
     next 
       \<comment>\<open>Failure case\<close>
       assume "res = RFailure"
