ViperBoogieFunctionInst.thy
@@ -262,7 +262,7 @@ lemma ctxt_wf_fun_interp:
 lemma assume_state_normal:
   assumes CtxtWf: "ctxt_wf Pr TyRep F FunMap ctxt" and
           FieldTr: "field_translation Tr = F" and
-          StateRel: "state_rel Pr TyRep Tr AuxPred ctxt \<omega> ns" and 
+          StateRel: "state_rel Pr TyRep Tr AuxPred ctxt \<omega>def \<omega> ns" and 
           Heq: "heap_var Tr = h" and
           Meq: "mask_var Tr = m" and
           StateName: "FunMap FGoodState = state_name"
