ViperBoogieRelUtil.thy
@@ -6,21 +6,21 @@ subsection \<open>Temporary variable management\<close>
 
 lemma store_temporary_var:
   assumes
-  StateRel: "state_rel Pr TyRep Tr AuxPred ctxt \<omega> ns" (is "?R \<omega> ns") and
+  StateRel: "state_rel Pr TyRep Tr AuxPred ctxt \<omega>def \<omega> ns" (is "?R \<omega> ns") and
          TyInterp:  "type_interp ctxt = vbpl_absval_ty TyRep" and
-         DisjAux: "temp_var \<notin> {heap_var Tr, mask_var Tr} \<union> ran (var_translation Tr) \<union> 
+         DisjAux: "temp_var \<notin> {heap_var Tr, mask_var Tr, heap_var_def Tr, mask_var_def Tr} \<union> ran (var_translation Tr) \<union> 
                      ran (field_translation Tr) \<union> range (const_repr Tr) \<union> dom AuxPred" and
          LookupTyTemp: "lookup_var_ty (var_context ctxt) temp_var = Some \<tau>_bpl" and
          RedRhs:  "red_expr_bpl ctxt e ns v" and
          TyValBpl:  "type_of_val (type_interp ctxt) v = \<tau>_bpl"
    shows "\<exists>ns'. red_ast_bpl P ctxt (((BigBlock name (Lang.Assign temp_var e # cs) s tr), cont), Normal ns)
                                    ((BigBlock name cs s tr, cont), Normal ns') \<and>
-                (state_rel Pr TyRep Tr (AuxPred(temp_var \<mapsto> pred_eq v)) ctxt \<omega> ns')"
+                (state_rel Pr TyRep Tr (AuxPred(temp_var \<mapsto> pred_eq v)) ctxt \<omega>def \<omega> ns')"
            (is "\<exists>ns'. ?red ns' \<and> ?R' \<omega> ns'")
 proof (rule exI, rule conjI)
   let ?ns' = "update_var (var_context ctxt) ns temp_var v"
 
-  have StateRel2: "state_rel Pr TyRep Tr (AuxPred(temp_var \<mapsto> pred_eq v)) ctxt \<omega> ?ns'"
+  have StateRel2: "state_rel Pr TyRep Tr (AuxPred(temp_var \<mapsto> pred_eq v)) ctxt \<omega>def \<omega> ?ns'"
     using state_rel_new_auxvar[OF \<open>?R \<omega> ns\<close> DisjAux _ TyInterp LookupTyTemp] TyValBpl
     unfolding pred_eq_def
     by simp    
@@ -36,17 +36,17 @@ qed
 
 lemma store_vpr_exp_to_temporary_var:
   assumes  
-  StateRel: "state_rel Pr TyRep Tr AuxPred ctxt \<omega> ns" (is "?R \<omega> ns") and
+  StateRel: "state_rel Pr TyRep Tr AuxPred ctxt \<omega>def \<omega> ns" (is "?R \<omega>def \<omega> ns") and
          TyInterp:  "type_interp ctxt = vbpl_absval_ty TyRep" and
-         DisjAux: "temp_var \<notin> {heap_var Tr, mask_var Tr} \<union> ran (var_translation Tr) \<union> 
+         DisjAux: "temp_var \<notin> {heap_var Tr, mask_var Tr, heap_var_def Tr, mask_var_def Tr} \<union> ran (var_translation Tr) \<union> 
                      ran (field_translation Tr) \<union> range (const_repr Tr) \<union> dom AuxPred" and
          LookupTyTemp: "lookup_var_ty (var_context ctxt) temp_var = Some \<tau>_bpl" and
-  RedRhsVpr:  "ctxt_vpr, StateCons, Some \<omega> \<turnstile> \<langle>e_vpr;\<omega>\<rangle> [\<Down>]\<^sub>t Val v" and
-  ExpRel: "exp_rel_vpr_bpl (state_rel_ext (state_rel Pr TyRep Tr AuxPred ctxt)) ctxt_vpr ctxt e_vpr e_bpl" and
+  RedRhsVpr:  "ctxt_vpr, StateCons, Some \<omega>def \<turnstile> \<langle>e_vpr;\<omega>\<rangle> [\<Down>]\<^sub>t Val v" and
+  ExpRel: "exp_rel_vpr_bpl (state_rel Pr TyRep Tr AuxPred ctxt) ctxt_vpr ctxt e_vpr e_bpl" and
          TyValBpl:  "type_of_val (type_interp ctxt) (val_rel_vpr_bpl v) = \<tau>_bpl"
    shows "\<exists>ns'. red_ast_bpl P ctxt (((BigBlock name (Lang.Assign temp_var e_bpl # cs) s tr), cont), Normal ns)
                                    ((BigBlock name cs s tr, cont), Normal ns') \<and>
-                (state_rel Pr TyRep Tr (AuxPred(temp_var \<mapsto> pred_eq (val_rel_vpr_bpl v))) ctxt \<omega> ns')"
+                (state_rel Pr TyRep Tr (AuxPred(temp_var \<mapsto> pred_eq (val_rel_vpr_bpl v))) ctxt \<omega>def \<omega> ns')"
 proof (rule store_temporary_var[OF StateRel TyInterp DisjAux LookupTyTemp _ TyValBpl])
   show "red_expr_bpl ctxt e_bpl ns (val_rel_vpr_bpl v)"
     using exp_rel_vpr_bpl_elim_2[OF ExpRel] RedRhsVpr StateRel
@@ -55,16 +55,16 @@ qed
 
 lemma store_temporary_perm_rel:
   assumes
-  StateRel: "state_rel Pr TyRep Tr AuxPred ctxt \<omega> ns" (is "?R \<omega> ns") and
-  RedPerm:  "ctxt_vpr, StateCons, Some \<omega> \<turnstile> \<langle>e_vpr;\<omega>\<rangle> [\<Down>]\<^sub>t Val (VPerm p)" and
-  ExpRel: "exp_rel_vpr_bpl (state_rel_ext (state_rel Pr TyRep Tr AuxPred ctxt)) ctxt_vpr ctxt e_vpr e_bpl" and
-         DisjAux: "temp_var \<notin> {heap_var Tr, mask_var Tr} \<union> ran (var_translation Tr) \<union> 
+  StateRel: "state_rel Pr TyRep Tr AuxPred ctxt \<omega>def \<omega> ns" (is "?R \<omega>def \<omega> ns") and
+  RedPerm:  "ctxt_vpr, StateCons, Some \<omega>def \<turnstile> \<langle>e_vpr;\<omega>\<rangle> [\<Down>]\<^sub>t Val (VPerm p)" and
+  ExpRel: "exp_rel_vpr_bpl (state_rel Pr TyRep Tr AuxPred ctxt) ctxt_vpr ctxt e_vpr e_bpl" and
+         DisjAux: "temp_var \<notin> {heap_var Tr, mask_var Tr, heap_var_def Tr, mask_var_def Tr} \<union> ran (var_translation Tr) \<union> 
                      ran (field_translation Tr) \<union> range (const_repr Tr) \<union> dom AuxPred" and
          LookupTyTemp: "lookup_var_ty (var_context ctxt) temp_var = Some (TPrim TReal)" and
          TyInterp:  "type_interp ctxt = vbpl_absval_ty TyRep"
   shows "\<exists>ns'. red_ast_bpl P ctxt (((BigBlock name (Lang.Assign temp_var e_bpl # cs) s tr), cont), Normal ns)
                                    ((BigBlock name cs s tr, cont), Normal ns') \<and>
-                (state_rel Pr TyRep Tr (AuxPred(temp_var \<mapsto> pred_eq (RealV (real_of_rat p)))) ctxt \<omega> ns')"
+                (state_rel Pr TyRep Tr (AuxPred(temp_var \<mapsto> pred_eq (RealV (real_of_rat p)))) ctxt \<omega>def \<omega> ns')"
            (is "\<exists>ns'. ?red ns' \<and> ?R' \<omega> ns'")
    using store_vpr_exp_to_temporary_var[OF StateRel TyInterp DisjAux LookupTyTemp RedPerm ExpRel]
    by simp
@@ -73,19 +73,24 @@ subsection \<open>Permission checks\<close>
 
 lemma pos_perm_rel_nontrivial:
   assumes "zero_perm = const_repr Tr CNoPerm" and
+          StateRelImpl:"\<And> \<omega>def \<omega> ns. R \<omega>def \<omega> ns \<Longrightarrow> state_rel Pr TyRep Tr (AuxPred(temp_perm \<mapsto> pred_eq (RealV (real_of_rat p)))) ctxt \<omega>def \<omega> ns" and
           SuccessCond:"\<And> \<omega> \<omega>'. Success \<omega> \<omega>' \<Longrightarrow> \<omega> = \<omega>' \<and> p \<ge> 0" and
           FailCond: "\<And> \<omega>. Fail \<omega> \<Longrightarrow> p < 0"
-shows "rel_general (state_rel Pr TyRep Tr (AuxPred(temp_perm \<mapsto> pred_eq (RealV (real_of_rat p)))) ctxt)
-                   (state_rel Pr TyRep Tr (AuxPred(temp_perm \<mapsto> pred_eq (RealV (real_of_rat p)))) ctxt)
+shows "rel_general (uncurry R) 
+                   (uncurry R)
      Success Fail
      P ctxt
      (BigBlock name (cmd.Assert (expr.Var temp_perm \<guillemotleft>Ge\<guillemotright> expr.Var zero_perm) # cs) s tr, cont)
      (BigBlock name cs s tr, cont)" (is "rel_general ?R ?R ?Success ?Fail P ctxt ?\<gamma> ?\<gamma>'")
 proof (rule assert_single_step_rel[where ?cond="\<lambda>_. p \<ge> 0"])
-  fix \<omega> ns
-  assume StateRel: "state_rel Pr TyRep Tr (AuxPred(temp_perm \<mapsto> pred_eq (RealV (real_of_rat p)))) ctxt \<omega> ns"
+  fix \<omega>def_\<omega> ns
+  
+  assume "uncurry R \<omega>def_\<omega> ns" 
+  hence StateRel: "state_rel Pr TyRep Tr (AuxPred(temp_perm \<mapsto> pred_eq (RealV (real_of_rat p)))) ctxt (fst \<omega>def_\<omega>) (snd \<omega>def_\<omega>) ns"
+    using StateRelImpl
+    by simp
   let ?p_bpl = "RealV (real_of_rat p)"
-
+  
   have LookupTempPerm: "lookup_var (var_context ctxt) ns temp_perm = Some ?p_bpl"
     using state_rel_aux_pred_sat_lookup_2[OF StateRel]
     unfolding pred_eq_def
@@ -93,7 +98,7 @@ proof (rule assert_single_step_rel[where ?cond="\<lambda>_. p \<ge> 0"])
   thus "red_expr_bpl ctxt (expr.Var temp_perm \<guillemotleft>Ge\<guillemotright> expr.Var zero_perm) ns (BoolV (0 \<le> p))"
         by (auto intro!: red_expr_red_exprs.intros                         
              intro: LookupTempPerm
-                    boogie_const_rel_lookup[OF state_rel0_boogie_const[OF state_rel_state_rel0[OF StateRel]]]
+                    boogie_const_rel_lookup[OF state_rel0_boogie_const_rel[OF state_rel_state_rel0[OF StateRel]]]
              simp: \<open>zero_perm = _\<close> )
 qed (insert assms, auto)
 
